tuning; moving;

Weidenbach_Book/IsaSAT_Arena.thy
@@ -1475,11 +1475,11 @@ lemma arena_dom_status_iff:
   assumes valid: \<open>valid_arena arena N vdom\<close> and
    i: \<open>i \<in> vdom\<close>
   shows
-     \<open>i \<in># dom_m N \<longleftrightarrow> arena_status arena i \<noteq> DELETED\<close> (is \<open>?eq\<close> is \<open>?A \<longleftrightarrow> ?B\<close>) and
-     \<open>is_LBD (arena ! (i - LBD_SHIFT))\<close> (is ?lbd) and
-     \<open>is_Act (arena ! (i - ACTIVITY_SHIFT))\<close> (is ?act) and
-     \<open>is_Status (arena ! (i - STATUS_SHIFT))\<close> (is ?stat) and
-     \<open>4 \<le> i\<close> (is ?ge)
+    \<open>i \<in># dom_m N \<longleftrightarrow> arena_status arena i \<noteq> DELETED\<close> (is \<open>?eq\<close> is \<open>?A \<longleftrightarrow> ?B\<close>) and
+    \<open>is_LBD (arena ! (i - LBD_SHIFT))\<close> (is ?lbd) and
+    \<open>is_Act (arena ! (i - ACTIVITY_SHIFT))\<close> (is ?act) and
+    \<open>is_Status (arena ! (i - STATUS_SHIFT))\<close> (is ?stat) and
+    \<open>4 \<le> i\<close> (is ?ge)
 proof -
   have H1: ?eq ?lbd ?act ?stat ?ge
     if \<open>?A\<close>
@@ -1523,8 +1523,7 @@ proof -
       using arena_lifting[OF valid, of i] that
       by auto
   qed
-  moreover have ?lbd ?act ?stat ?ge
-    if \<open>\<not>?A\<close>
+  moreover have ?lbd ?act ?stat ?ge if \<open>\<not>?A\<close>
   proof -
     have
       \<open>arena_dead_clause (Misc.slice (i - 4) i arena)\<close> and
@@ -1562,8 +1561,8 @@ definition arena_is_valid_clause_vdom :: \<open>arena \<Rightarrow> nat \<Righta
 
 subsubsection \<open>Code Generation\<close>
 
-
 paragraph \<open>Length\<close>
+
 definition isa_arena_length where
   \<open>isa_arena_length arena i = do {
       ASSERT(i \<ge> SIZE_SHIFT \<and> i < length arena);
@@ -1639,6 +1638,22 @@ lemma isa_arena_length_code_refine[sepref_fr_rules]:
   unfolding hr_comp_assoc[symmetric] uncurry_def list_rel_compp
   by (simp add: arl_assn_comp)
 
+sepref_definition isa_arena_length_fast_code
+  is \<open>uncurry isa_arena_length\<close>
+  :: \<open>(arl_assn uint32_assn)\<^sup>k *\<^sub>a uint64_nat_assn\<^sup>k \<rightarrow>\<^sub>a uint64_assn\<close>
+  supply arena_el_assn_alt_def[symmetric, simp] sum_uint64_assn[sepref_fr_rules]
+    minus_uint64_nat_assn[sepref_fr_rules]
+  unfolding isa_arena_length_def SIZE_SHIFT_def fast_minus_def one_uint64_nat_def[symmetric]
+  by sepref
+
+lemma isa_arena_length_fast_code_refine[sepref_fr_rules]:
+  \<open>(uncurry isa_arena_length_fast_code, uncurry (RETURN \<circ>\<circ> arena_length))
+  \<in> [uncurry arena_is_valid_clause_idx]\<^sub>a
+    arena_assn\<^sup>k *\<^sub>a uint64_nat_assn\<^sup>k \<rightarrow> uint64_nat_assn\<close>
+  using isa_arena_length_fast_code.refine[FCOMP isa_arena_length_arena_length]
+  unfolding hr_comp_assoc[symmetric] uncurry_def list_rel_compp
+  by (simp add: arl_assn_comp)
+
 
 paragraph \<open>Literal at given position\<close>
 
@@ -1660,7 +1675,6 @@ sepref_definition isa_arena_lit_code
   unfolding isa_arena_lit_def
   by sepref
 
-declare isa_arena_lit_code.refine[sepref_fr_rules]
 
 lemma arena_length_literal_conv:
   assumes
@@ -1707,7 +1721,7 @@ definition arena_lit_pre where
   (\<exists>j. i \<ge> j \<and> arena_is_valid_clause_idx_and_access arena j (i - j))\<close>
 
 lemma isa_arena_lit_arena_lit:
-  \<open>(uncurry (isa_arena_lit), uncurry (RETURN oo arena_lit)) \<in>
+  \<open>(uncurry isa_arena_lit, uncurry (RETURN oo arena_lit)) \<in>
     [uncurry arena_lit_pre]\<^sub>f
      \<langle>uint32_nat_rel O arena_el_rel\<rangle>list_rel \<times>\<^sub>r nat_rel \<rightarrow> \<langle>unat_lit_rel\<rangle>nres_rel\<close>
   unfolding isa_arena_lit_def arena_lit_def
@@ -1726,11 +1740,29 @@ lemma isa_arena_lit_code_refine[sepref_fr_rules]:
   unfolding hr_comp_assoc[symmetric] uncurry_def list_rel_compp
   by (simp add: arl_assn_comp)
 
+sepref_definition (in-) isa_arena_lit_fast_code
+  is \<open>uncurry isa_arena_lit\<close>
+  :: \<open>(arl_assn uint32_assn)\<^sup>k *\<^sub>a uint64_nat_assn\<^sup>k \<rightarrow>\<^sub>a uint32_assn\<close>
+  supply arena_el_assn_alt_def[symmetric, simp] sum_uint64_assn[sepref_fr_rules]
+  unfolding isa_arena_lit_def
+  by sepref
+
+declare isa_arena_lit_fast_code.refine
+
+lemma isa_arena_lit_fast_code_refine[sepref_fr_rules]:
+  \<open>(uncurry isa_arena_lit_fast_code, uncurry (RETURN \<circ>\<circ> arena_lit))
+  \<in> [uncurry arena_lit_pre]\<^sub>a
+    arena_assn\<^sup>k *\<^sub>a uint64_nat_assn\<^sup>k \<rightarrow> unat_lit_assn\<close>
+  using isa_arena_lit_fast_code.refine[FCOMP isa_arena_lit_arena_lit]
+  unfolding hr_comp_assoc[symmetric] uncurry_def list_rel_compp
+  by (simp add: arl_assn_comp)
+
+
 
 paragraph \<open>Status of the clause\<close>
 
 
-lemma (in -) status_assn_hnr_eq[sepref_fr_rules]:
+lemma status_assn_hnr_eq[sepref_fr_rules]:
   \<open>(uncurry (return oo (=)), uncurry (RETURN oo (=))) \<in> status_assn\<^sup>k *\<^sub>a status_assn\<^sup>k \<rightarrow>\<^sub>a
     bool_assn\<close>
   by sepref_to_hoare (sep_auto simp: status_rel_def hr_comp_def uint32_nat_rel_def br_def
@@ -2051,8 +2083,7 @@ proof -
      using le j_ge unfolding length[symmetric] header_size_def
      by (auto split: if_splits simp: POS_SHIFT_def)
   show ?ge
-    using j_ge ge by (auto simp: SHIFTS_def header_size_def is_short_clause_def
-        split: if_splits)
+    using j_ge ge by (auto simp: SHIFTS_def header_size_def split: if_splits)
   have
     \<open>(a ! (j - POS_SHIFT),
          (arena ! (j - POS_SHIFT)))
@@ -2131,6 +2162,7 @@ lemma isa_get_saved_pos_get_saved_pos':
       list_rel_imp_same_length get_saved_pos_pre_def
       intro!: ASSERT_leI)
 
+(* TODO check if we use this version anywhere *)
 lemma get_saved_pos_code':
   \<open>(uncurry isa_get_saved_pos_code, uncurry (RETURN \<circ>\<circ> arena_pos))
      \<in> [uncurry get_saved_pos_pre]\<^sub>a arena_assn\<^sup>k *\<^sub>a nat_assn\<^sup>k \<rightarrow> nat_assn\<close>
@@ -2138,20 +2170,41 @@ lemma get_saved_pos_code':
   unfolding hr_comp_assoc[symmetric] list_rel_compp status_assn_alt_def uncurry_def
   by (auto simp add: arl_assn_comp update_lbd_pre_def)
 
+lemma (in -) POS_SHIFT_uint64_hnr:
+  \<open>(uncurry0 (return 5), uncurry0 (RETURN POS_SHIFT)) \<in> unit_assn\<^sup>k \<rightarrow>\<^sub>a uint64_nat_assn\<close>
+  by sepref_to_hoare (sep_auto simp: POS_SHIFT_def uint64_nat_rel_def br_def)
+
+
+sepref_definition isa_get_saved_pos_fast_code2
+  is \<open>uncurry isa_get_saved_pos\<close>
+  :: \<open>(arl_assn uint32_assn)\<^sup>k *\<^sub>a uint64_nat_assn\<^sup>k \<rightarrow>\<^sub>a uint64_assn\<close>
+  supply sum_uint64_assn[sepref_fr_rules] POS_SHIFT_uint64_hnr[sepref_fr_rules]
+  unfolding isa_get_saved_pos_def
+  by sepref
+
+lemma get_saved_pos_code2[sepref_fr_rules]:
+  \<open>(uncurry isa_get_saved_pos_fast_code2, uncurry (RETURN \<circ>\<circ> arena_pos))
+     \<in> [uncurry get_saved_pos_pre]\<^sub>a arena_assn\<^sup>k *\<^sub>a uint64_nat_assn\<^sup>k \<rightarrow> uint64_nat_assn\<close>
+  using isa_get_saved_pos_fast_code2.refine[FCOMP isa_get_saved_pos_get_saved_pos]
+  unfolding hr_comp_assoc[symmetric] list_rel_compp status_assn_alt_def uncurry_def
+  by (auto simp add: arl_assn_comp update_lbd_pre_def)
+
 
 paragraph \<open>Update Saved Position\<close>
 
-(* TODO: converting to uint32 is a little stupid and always useless (uint64 is enough everytime) *)
+(* TODO: converting from nat to uint32 is a little stupid and always useless (uint64 is enough everytime) *)
 definition isa_update_pos :: \<open>nat \<Rightarrow> nat \<Rightarrow> uint32 list \<Rightarrow> uint32 list nres\<close> where
-  \<open>isa_update_pos C lbd arena = do {
-      ASSERT(C - POS_SHIFT < length arena \<and> C \<ge> POS_SHIFT \<and> lbd \<ge> 2 \<and> lbd - 2 \<le> uint32_max);
-      RETURN (arena [C - POS_SHIFT := (uint32_of_nat (lbd - 2))])
+  \<open>isa_update_pos C n arena = do {
+      ASSERT(C - POS_SHIFT < length arena \<and> C \<ge> POS_SHIFT \<and> n \<ge> 2 \<and> n - 2 \<le> uint32_max);
+      RETURN (arena [C - POS_SHIFT := (uint32_of_nat (n - 2))])
   }\<close>
 
+(* TODO Move *)
 lemma (in -) uint32_of_nat[sepref_fr_rules]:
   \<open>(return o uint32_of_nat, RETURN o uint32_of_nat) \<in> [\<lambda>n. n \<le> uint32_max]\<^sub>a nat_assn\<^sup>k \<rightarrow> uint32_assn\<close>
   by sepref_to_hoare
     sep_auto
+(* End Move *)
 
 sepref_definition isa_update_pos_code
   is \<open>uncurry2 isa_update_pos\<close>
@@ -2246,6 +2299,82 @@ lemma isa_update_pos_code_hnr[sepref_fr_rules]:
 lemma MAX_LENGTH_SHORT_CLAUSE_hnr[sepref_fr_rules]:
   \<open>(uncurry0 (return 5), uncurry0 (RETURN MAX_LENGTH_SHORT_CLAUSE)) \<in> unit_assn\<^sup>k \<rightarrow>\<^sub>a uint64_nat_assn\<close>
   by sepref_to_hoare (sep_auto simp: uint64_nat_rel_def br_def)
+
+
+paragraph \<open>Mark clause as garbage\<close>
+
+definition mark_garbage_pre where
+  \<open>mark_garbage_pre = (\<lambda>(arena, C). arena_is_valid_clause_idx arena C)\<close>
+
+definition mark_garbage where
+  \<open>mark_garbage arena C = do {
+    ASSERT(C \<ge> STATUS_SHIFT \<and> C - STATUS_SHIFT < length arena);
+    RETURN (arena[C - STATUS_SHIFT := (3 :: uint32)])
+  }\<close>
+
+lemma mark_garbage_pre:
+  assumes 
+    j: \<open>j \<in># dom_m N\<close> and
+    valid: \<open>valid_arena arena N x\<close> and
+    arena: \<open>(a, arena) \<in> \<langle>uint32_nat_rel O arena_el_rel\<rangle>list_rel\<close>
+  shows
+    \<open>STATUS_SHIFT \<le> j\<close> (is ?ge) and
+    \<open>(a[j - STATUS_SHIFT := 3], arena[j - STATUS_SHIFT := AStatus DELETED])
+         \<in> \<langle>uint32_nat_rel O arena_el_rel\<rangle>list_rel\<close> (is ?rel) and
+    \<open>j - STATUS_SHIFT < length arena\<close> (is ?le)
+proof -
+  have j_le: \<open>j < length arena\<close> and
+    length: \<open>length (N \<propto> j) = arena_length arena j\<close> and
+    k1:\<open>\<And>k. k < length (N \<propto> j) \<Longrightarrow> N \<propto> j ! k = arena_lit arena (j + k)\<close> and
+    k2:\<open>\<And>k. k < length (N \<propto> j) \<Longrightarrow> is_Lit (arena ! (j+k))\<close> and
+    le: \<open>j + length (N \<propto> j) \<le> length arena\<close>  and
+    j_ge: \<open>header_size (N \<propto> j) \<le> j\<close>
+    using arena_lifting[OF valid j] by (auto simp: )
+  show le': ?le
+     using le j_ge unfolding length[symmetric] header_size_def
+     by (auto split: if_splits simp: SHIFTS_def)
+
+  show ?rel
+     apply (rule list_rel_update'[OF arena])
+     using length
+     by
+      (auto simp: arena_el_rel_def unat_lit_rel_def arena_lit_def update_lbd_def
+        uint32_nat_rel_def br_def Collect_eq_comp status_rel_def
+       split: arena_el.splits
+       intro!: )
+
+  show ?ge
+     using le j_ge unfolding length[symmetric] header_size_def
+     by (auto split: if_splits simp: SHIFTS_def)
+qed
+
+sepref_definition mark_garbage_code
+  is \<open>uncurry mark_garbage\<close>
+  :: \<open>(arl_assn uint32_assn)\<^sup>d *\<^sub>a nat_assn\<^sup>k \<rightarrow>\<^sub>a arl_assn uint32_assn\<close>
+  unfolding mark_garbage_def
+  by sepref
+
+lemma isa_mark_garbage:
+  \<open>(uncurry mark_garbage, uncurry (RETURN oo extra_information_mark_to_delete)) \<in>
+    [mark_garbage_pre]\<^sub>f
+     \<langle>uint32_nat_rel O arena_el_rel\<rangle>list_rel \<times>\<^sub>f nat_rel  \<rightarrow>
+    \<langle>\<langle>uint32_nat_rel O arena_el_rel\<rangle>list_rel\<rangle>nres_rel\<close>
+  unfolding isa_arena_status_def arena_status_def
+  by (intro frefI nres_relI)
+    (auto simp: arena_is_valid_clause_idx_def uint64_nat_rel_def br_def two_uint64_def
+        list_rel_imp_same_length arena_length_uint64_conv arena_lifting
+        arena_is_valid_clause_idx_and_access_def arena_lbd_conv
+        arena_is_valid_clause_vdom_def arena_status_literal_conv mark_garbage_pre
+        mark_garbage_def mark_garbage_pre_def extra_information_mark_to_delete_def
+        isa_arena_swap_def swap_lits_def swap_lits_pre_def isa_update_lbd_def
+      intro!: ASSERT_refine_left)
+
+lemma mark_garbage_hnr[sepref_fr_rules]:
+  \<open>(uncurry mark_garbage_code, uncurry (RETURN oo extra_information_mark_to_delete))
+  \<in> [mark_garbage_pre]\<^sub>a  arena_assn\<^sup>d *\<^sub>a nat_assn\<^sup>k \<rightarrow> arena_assn\<close>
+  using mark_garbage_code.refine[FCOMP isa_mark_garbage]
+  unfolding hr_comp_assoc[symmetric] list_rel_compp status_assn_alt_def uncurry_def
+  by (auto simp add: arl_assn_comp update_lbd_pre_def)
 
 
 end
